Written TM2 code. Yet to prove correctness

src/computability/is_odd.lean
@@ -1,4 +1,5 @@
 import tactic
+import data.list
 import .problem
 
 namespace tm2program
@@ -9,29 +10,34 @@ open problem
 section
 
 inductive K₀
-| nat_to_list_aux
+| t1 | t2
+parameters {K : Type*} [decidable_eq K] -- Index type of stacks
+parameters (lK : K₀ → K)
+parameters (k₀ : K) -- input stack
+parameters (k₁ : K) -- output stack
+parameters (k₂ : K) -- call stack
+parameters (h₀₂: k₀ ≠ k₂) -- input stack is not the call stack
 
 @[derive decidable_eq]
 inductive vars₀
 | temp
 open vars₀
-
-inductive Λ₀
-| nat_to_list₁ ( n : ℕ ) ( f : K₀ ) ( t : K₀ )
-open Λ₀
-
-
-parameters {K : Type*} [decidable_eq K] -- Index type of stacks
-parameters (k₀ : K) -- input stack
-parameters (lK : K₀ → K)
-
-parameters (Λ : Type*) -- Type of function labels
-parameters (lΛ : Λ₀ → Λ)
-parameters (vars : Type) [decidable_eq vars]
+parameters {vars : Type} [decidable_eq vars]
 parameters (lv : vars₀ → vars) 
 
+inductive Λ₀
+| copy_rec ( f : K ) ( t : K ) ( n : fin 2 ) 
+| copy_rec₂ ( f : K ) ( t : K ) ( n : fin 1 ) 
+| pop_rec ( t : K ) ( n : fin 1 ) 
+| list_head ( f : K ) ( t : K ) ( n : fin 2 ) 
+| nat_to_list₂ ( f : K ) ( t : K ) ( n : fin 1 )  
+open Λ₀
 
-def σ := vars → option Γ' 
+parameters (Λ : Type) -- Type of function labels
+parameters (lΛ : Λ₀ → Λ)
+
+def σ := (vars → option Γ') × Λ 
+
 
 /-
 inductive stmt
@@ -46,43 +52,173 @@ open stmt
 -/
 
 -- inductive Γ' | blank | bit0 | bit1 | left | right | comma
+def Γ: K → Type := λ k, if k = k₂ then Λ else Γ'
 
-def Γ : K → Type := λ k : K, Γ' 
 
-def s := stmt Γ Λ σ 
+
+def stmt' := turing.TM2.stmt Γ Λ σ 
 --inductive Γ' | blank | bit0 | bit1 | bra | ket | comma 
 
--- def const : K₀ → σ → Γ' := λ t _, t 
-
-def set_var : vars₀ → σ → option Γ' → σ := λ v f s x, if lv v = x then s else f x
+/-def set_var : vars₀ → σ → option Γ' → σ := λ v f s x, if lv v = x then s else f x
 def get_var : vars₀ → Γ' → σ → Γ' := λ v d f, option.cases_on (f(lv v)) d (λ x, x) 
 def get_var' : vars₀ → σ → Γ' := λ v, get_var v Γ'.blank 
 def ignore : σ → option Γ' → σ := λ f _, f
-def goto' : Λ₀ → stmt Γ Λ σ  := λ l, goto (λ _, lΛ (l) )
+def goto' : Λ₀ → stmt'  := λ l, goto (λ _, lΛ (l) )
+def var_eq : vars₀ → Γ' → σ → bool := λ v x f, f (lv v) = x
+def var_undef : vars₀ → σ → bool := λ v f, f (lv v) = none-/
 
-def func_nat_to_list₁ ( f : K₀ ) ( t : K₀ ) : ℕ → stmt Γ Λ σ 
-| 0 :=
-   pop (lK f) ignore $
-   pop (lK t) ignore $
-   push (lK t) ( λ _, Γ'.comma ) $
-   push (lK t) ( λ _, Γ'.ket ) $
-   goto' $ nat_to_list₁ 1 f t
-| 1 := 
-   pop (lK f) (set_var temp) $
-   branch ( λ f:σ, f (lv temp) = Γ'.comma ) (
-      goto' $ nat_to_list₁ 1 f t
-   ) (
-      push (lK t) ( λ _, Γ'.comma ) $
-      push (lK t) (get_var' temp) $ 
-      goto' $ nat_to_list₁ 2 f t
-   ) 
+--attribute [class] ne
+
+/-lemma ne_call_stack {k:K} (h:k≠k₂): Γ k = Γ' :=
+begin
+   change (if k = k₂ then Λ else Γ') = Γ',
+   simp [h],
+end
+def push_const {k:K} (h:k≠k₂) : Γ' → stmt' → stmt' := λ g e, push k ( λ σ, begin
+   rw ne_call_stack k₂ Λ h,
+   exact g,
+end ) e 
+def pop' {k:K} (h:k≠k₂) : (σ → option Γ' → σ) → stmt' → stmt' := λ f e, pop k begin 
+   rw ne_call_stack k₂ Λ h,
+   exact f, 
+end e -/
+
+def no_call_stack: K → K := λ k, if k=k₂ then k₀ else k
+include h₀₂
+lemma no_call_stack_elim (k:K): Γ ( no_call_stack k ) = Γ' :=
+begin
+   change (if (if k=k₂ then k₀ else k) = k₂ then Λ else Γ') = Γ',
+   cases _inst_1 k k₂ with h h, simp [h],
+   exact if_neg h₀₂,
+end
+def no_option: option Γ' → Γ' := λ l, option.cases_on l Γ'.blank id 
+
+-- syntactic sugar
+def push_const: K → Γ' → stmt' → stmt' := λ k g e, push (no_call_stack k) (λ f,by{ rw no_call_stack_elim _ _ h₀₂, use g,}) e
+def push_var: K → vars → stmt' → stmt' := λ k v e, push (no_call_stack k) (λ f,by{ rw no_call_stack_elim _ _ h₀₂, use no_option _ _ h₀₂ (f.1 v),}) e
+def discard: K → stmt' → stmt' := λ k e, pop k (λ f g, f) e
+def pop_var: K → vars → stmt' → stmt' := λ k v e, pop (no_call_stack k) (λ f g, (λ w, if v = w then by{ rw ← no_call_stack_elim _ _ h₀₂, use g, } else f.1 w, f.2)) e 
+def goto' : Λ₀ → stmt'  := λ l, goto (λ _, lΛ (l) )
+def var_eq_const : vars → Γ' → σ → bool := λ v x f, f.1 v = x
+def var_undef : vars → σ → bool := λ v f, f.1 v = none
+def call : Λ → Λ → stmt' := λ a b, push k₂ (λ f, begin 
+   change (if k₂ = k₂ then Λ else Γ'),
+   simp,
+   use b,
+end) $ goto (λ _, a)
+def return : stmt' := pop k₂ begin
+   intros f g,
+   change option (if k₂ = k₂ then Λ else Γ') at g,
+   simp at g,
+   cases g, use f,
+   use (f.1,g),
+end $ goto (λ f, f.2)
+
+-- programs
+
+def func_nat_to_list₂ (f:K) (t:K): ℕ → stmt Γ Λ σ 
+| 0 := 
+   push_const t Γ'.comma $ 
+   push_const t Γ'.ket $
+   goto' $ nat_to_list₂ f t 1
 | _ := 
-   push (lK t) ( λ _, Γ'.bra ) $
-   push (lK t) ( λ _, Γ'.bra ) $
-   pop (lK f) ignore $
-   push (lK f) ( λ _, Γ'.bra ) $
-   halt 
+   pop_var f (lv temp) $
+   branch (var_eq_const (lv temp) Γ'.comma) (
+      push_const t Γ'.bra $
+      return 
+   ) (
+      push_const t Γ'.comma $
+      push_var t (lv temp) $ 
+      goto' $ nat_to_list₂ f t 1
+   ) 
 
+/-def func_nat_to_list₂ (f:K) (t:K) (t₂:t≠k₂) (f₂:f≠k₂): ℕ → stmt Γ Λ σ 
+| 0 := 
+   push_const t₂ Γ'.comma $ 
+   push_const t₂ Γ'.ket $
+   goto' $ nat_to_list₂ f t 1
+| _ := 
+   pop' f₂ (set_var temp) $
+   branch (var_eq temp Γ'.comma) (
+      push_const t₂ Γ'.bra $
+      halt 
+   ) (
+      push_const t₂ Γ'.comma $
+      push_var t₂ temp $ 
+      goto' $ nat_to_list₂ f t 1
+   ) -/
+
+-- f = t is not allowed, reverses
+def func_copy_rec₂ (f : K) (t : K): ℕ → stmt Γ Λ σ 
+| 0 := 
+   push_const (lK K₀.t1) Γ'.comma $
+   goto' $ copy_rec₂ f t 1
+| _ := 
+   pop_var f (lv temp) $
+   branch (var_eq_const (lv temp) Γ'.bra) (
+      push_const t Γ'.ket $
+      push_const t Γ'.comma $
+      push_const (lK K₀.t1) Γ'.bit1 $
+      goto' $ copy_rec₂ f t 1
+   ) $
+   branch (var_eq_const (lv temp) Γ'.ket) (
+      discard t $
+      push_const t Γ'.bra $
+      discard (lK K₀.t1) $
+      goto' $ copy_rec₂ f t 1
+   ) $
+   branch (var_eq_const (lv temp) Γ'.comma) (
+      push_const t Γ'.comma $
+      pop_var (lK K₀.t1) (lv temp) $
+      branch (var_eq_const (lv temp) Γ'.bit1) (
+         goto' $ copy_rec₂ f t 1
+      ) $
+      return
+   ) $
+   push_var t (lv temp) $
+   goto' $ copy_rec₂ f t 1
+
+-- f = t is allowed, does not reverse
+def func_copy_rec (f : K) (t : K): ℕ → stmt Γ Λ σ 
+| 0 :=   call (lΛ (copy_rec₂ f (lK K₀.t2) 0) ) (lΛ (copy_rec f t 1) )
+| 1 :=   call (lΛ (copy_rec₂ (lK K₀.t2) t 0) ) (lΛ (copy_rec f t 2) )
+| _ :=   return
+
+def func_pop_rec (f : K): ℕ → stmt Γ Λ σ 
+| 0 := 
+   push_const (lK K₀.t1) Γ'.comma $
+   goto' $ pop_rec f 1
+| _ := 
+   pop_var f (lv temp) $
+   branch (var_eq_const (lv temp) Γ'.bra) (
+      push_const (lK K₀.t1) Γ'.bit1 $
+      goto' $ pop_rec f 1
+   ) $
+   branch (var_eq_const (lv temp) Γ'.ket) (
+      discard (lK K₀.t1) $
+      goto' $ pop_rec f 1
+   ) $
+   branch (var_eq_const (lv temp) Γ'.comma) (
+      pop_var (lK K₀.t1) (lv temp) $
+      branch (var_eq_const (lv temp) Γ'.bit1) (
+         goto' $ pop_rec f 1
+      ) $
+      return
+   ) $
+   goto' $ pop_rec f 1
+
+/-def func_clear_stack (t : K): ℕ → stmt Γ Λ σ 
+| _ := 
+   pop_var t (lv temp) $
+   branch (var_undef (lv temp)) return $
+   goto' $ clear_stack t 0-/
+
+def func_list_head (f : K) (t : K): ℕ → stmt Γ Λ σ 
+| 0 :=   discard f $
+         call (lΛ (copy_rec f t 0)) (lΛ (list_head f t 1))
+| 1 :=   push_const f Γ'.bra $
+         call (lΛ (pop_rec f 0)) (lΛ (list_head f t 2))
+| _ :=   return
 
 end
 end tm2program
